theories/microgv/TODO.md
@@ -1,7 +1,4 @@
 TODO:
-* linv_out_Some
-* expr_refs_linv
 * graph lemma
 * preservation proof
-* progress proof 2 admits
 * encode session types
